src/drf/PFSingle.v
@@ -20,7 +20,6 @@ Require Import Thread.
 Require Import Configuration.
 Require Import Progress.
 Require Import Behavior.
-Require Import Race.
 
 Require Import PF.
 
